translated a post-condition

leetcde_283_with_hax/src/main.rs
@@ -1,10 +1,13 @@
 const MAX_SIZE: usize = 100; // maximum number of kids
 
-pub fn kids_with_candies(candies: [i32; MAX_SIZE], extra_candies: i32, l: usize) -> [i32; MAX_SIZE] {
+
+
+#[hax_lib::ensures(|result| result.len()==MAX_SIZE)]
+pub fn kids_with_candies(candies: [i32; MAX_SIZE], extra_candies: i32) -> [i32; MAX_SIZE] {
     let mut candies_max = candies[0];
 
-    // Find the maximum candy count
-    for i in 0..l {
+    // Find the maximum candy count in vector
+    for i in 0..MAX_SIZE {
         if candies[i] > candies_max {
             candies_max = candies[i];
         }
@@ -14,7 +17,7 @@ pub fn kids_with_candies(candies: [i32; MAX_SIZE], extra_candies: i32, l: usize)
     let mut will_have_greatest = [0; MAX_SIZE];
 
     // Fill the result array
-    for i in 0..l {
+    for i in 0..MAX_SIZE {
         if candies[i] + extra_candies >= candies_max {
             will_have_greatest[i] = 1;
         }
@@ -23,8 +26,11 @@ pub fn kids_with_candies(candies: [i32; MAX_SIZE], extra_candies: i32, l: usize)
     will_have_greatest
 }
 
-fn main() {
-
+fn main (){
+    
 }
-
 //while loops, and methods both cause issues in lean translation.
+
+//sucessful translation requires for loops instead of while loop.
+//no methods
+//arrays instead of vectors
