leetcde_283_with_hax/proofs/lean/extraction/Leetcde_283_with_hax.lean
@@ -14,17 +14,33 @@ set_option linter.unusedVariables false
 def Leetcde_283_with_hax.MAX_SIZE : usize :=
   Result.of_isOk (do (pure (100 : usize))) (by rfl)
 
+def Leetcde_283_with_hax._.future
+  (T : Type) (x : T)
+  : Result (Rust_primitives.Hax.Tuple2 T T)
+  := do
+  let hax_temp_output : T := x;
+  (pure (Rust_primitives.Hax.Tuple2.mk x hax_temp_output))
+
+def Leetcde_283_with_hax._.ensures
+  (candies : (RustArray i32 100))
+  (extra_candies : i32)
+  (result : (RustArray i32 100))
+  : Result Bool
+  := do
+  (Rust_primitives.Hax.Machine_int.eq
+    (← (Core.Slice.Impl.len i32 (← (Rust_primitives.unsize result))))
+    Leetcde_283_with_hax.MAX_SIZE)
+
 def Leetcde_283_with_hax.kids_with_candies
   (candies : (RustArray i32 100))
   (extra_candies : i32)
-  (l : usize)
   : Result (RustArray i32 100)
   := do
   let candies_max : i32 ← candies[(0 : usize)]_?;
   let candies_max : i32 ←
     (Rust_primitives.Hax.Folds.fold_range
       (0 : usize)
-      l
+      Leetcde_283_with_hax.MAX_SIZE
       (fun candies_max _ => (do (pure true) : Result Bool))
       candies_max
       (fun candies_max i => (do
@@ -40,7 +56,7 @@ def Leetcde_283_with_hax.kids_with_candies
   let will_have_greatest : (RustArray i32 100) ←
     (Rust_primitives.Hax.Folds.fold_range
       (0 : usize)
-      l
+      Leetcde_283_with_hax.MAX_SIZE
       (fun will_have_greatest _ => (do (pure true) : Result Bool))
       will_have_greatest
       (fun will_have_greatest i => (do
@@ -63,3 +79,13 @@ def Leetcde_283_with_hax.main
   : Result Rust_primitives.Hax.Tuple0
   := do
   (pure Rust_primitives.Hax.Tuple0.mk)
+
+
+theorem kids_with_candies_len_correct :
+  ∀ (candies : RustArray i32 100) (extra_candies : i32),
+    ∀ result,
+      Leetcde_283_with_hax.kids_with_candies candies extra_candies = Result.ok result →
+      Leetcde_283_with_hax._.ensures candies extra_candies result = Result.ok true
+  := by sorry
+
+--this theorem would check the condition, but man this is kinda not so easy!
